\begin{figure}
  \bookmark{\PwTcTITLE{} Semantics}
  \raggedright
  
  \noindent
  If $\aPS \in \sSEMI{\aPSS_1}{\aPSS_2}$ then
  $(\exists\aPS_1\in\aPSS_1)$ $(\exists\aPS_2\in\aPSS_2)$
  $(\exists\phEvs_1\subseteq\AllEvents)$ $(\exists\phEvs_2\subseteq\AllEvents)$
  \begin{multicols}{2}
    \begin{enumerate}[topsep=0pt,label=(\textsc{s}\arabic*),ref=\textsc{s}\arabic*]
      \setcounter{enumi}{\value{BE}}
    \item \label{seq-E-phantom}
      $\aEvs=(\aEvs_1\cup\aEvs_2)\uplus\phEvs_1 \uplus\phEvs_2$,

    \item[\eqref{seq-lambda}]
      \eqref{seq-kappa}\;
      \eqref{seq-tau}\;
      \eqref{seq-term}\;
      \eqref{seq-le}\;
      as in \reffig{fig:seq},

      \setcounter{enumi}{\value{lambda}}
    \item[] 
      \begin{enumerate}[leftmargin=0pt]
      \item \label{seq-lambda-phantom1}
        if $\bEv\in \phEvs_1$ then $\labeling(\bEv)=\labeling_1(\fmrg{\bEv})$,
      \item \label{seq-lambda-phantom2}
        if $\bEv\in \phEvs_2$ then $\labeling(\bEv)=\labeling_2(\fmrg{\bEv})$,
      \end{enumerate}

      \setcounter{enumi}{\value{kappa}}
    \item[] 
      \begin{enumerate}[leftmargin=0pt]
        \setcounter{enumii}{3}
      \item \label{seq-kappa-phantom1}
        if $\bEv\in \phEvs_1$ then $\labelingForm(\bEv)\riff\labelingForm_1(\fmrg{\bEv})$,
      \item \label{seq-kappa-phantom2}
        if $\bEv\in \phEvs_2$ then $\labelingForm(\bEv)\riff\aTr[1]{}{\labelingForm_2(\fmrg{\bEv})}$,
      \end{enumerate}

      \columnbreak
      \setcounter{enumi}{\value{m}}
    \item[] \labeltext[\textsc{s}8]{}{seq-m}
      \begin{enumerate}[leftmargin=0pt]
      \item \label{seq-m-real-cup}
        if $\aEv\in(\aEvs_1\cup\aEvs_2)$ then $\fmrg{\aEv}=\aEv$,
      \item \label{seq-m-real-cap}
        if $\fmrg{\aEv}=\aEv$ then $\aEv\not\in(\aEvs_1\cap\aEvs_2)$,
      \item \label{seq-m-phantom-forall}
        if $\bEv\in (\phEvs_1\cup\phEvs_2)$ then
        $\fmrg{\bEv}\in (\aEvs_1\cap\aEvs_2)$,
      \item \label{seq-m-phantom-exists}
        if $\aEv\in (\aEvs_1\cap\aEvs_2)$ then
        $(\existsone\bEv_1\in\phEvs_1)$ $(\existsone\bEv_2\in\phEvs_1)$
        $\fmrg{\bEv_1}=\fmrg{\bEv_2}=\aEv$,
      \end{enumerate}

      \setcounter{enumi}{\value{Bpo}}
    \item \label{seq-po}
      if $\bEv\in\umEvs_1$ and $\aEv\in\umEvs_2$ then $\bEv\xpox\aEv$,
      
    \end{enumerate}
    where
    \makebox[0cm][l]{\begin{math}
      \umEvs_1= \phEvs_1 \cup (\aEvs_1\setminus\aEvs_2)
    \end{math}
    and
    \begin{math}
      \umEvs_2= \phEvs_2 \cup (\aEvs_2\setminus\aEvs_1).
    \end{math}}

  \end{multicols}
  \medskip

  \noindent
  If $\aPS \in \sIF{\aForm}\sTHEN\aPSS_1\sELSE\aPSS_2\sFI$ then
  $(\exists\aPS_1\in\aPSS_1)$ $(\exists\aPS_2\in\aPSS_2)$
  $(\exists\phEvs_1\subseteq\AllEvents)$ $(\exists\phEvs_2\subseteq\AllEvents)$
  \begin{multicols}{2}
    \begin{enumerate}[topsep=0pt,label=(\textsc{i}\arabic*),ref=\textsc{i}\arabic*]
    % \item[(\textsc{i}1)]
    %   (\textsc{i}2a)\;
    %   (\textsc{i}2b)\;
    %   (\textsc{i}8)\;
    %   (\textsc{i}9)\;
    %   as for $\sSEMI{}{}$,

    \item[\eqref{seq-E-phantom}]
      \eqref{seq-lambda-phantom1}\;
      \eqref{seq-lambda-phantom2}\;
      \eqref{seq-m}\;
      \eqref{seq-po}\;
      as for $\sSEMI{}{}$,

    \item[\eqref{if-lambda}]
      \eqref{if-kappa}\;
      \eqref{if-tau}\;
      \eqref{if-term}\; 
      \eqref{if-le}\;
      as in \reffig{fig:seq},

      \setcounter{enumi}{\value{kappa}}
    \item[] 
      \begin{enumerate}[leftmargin=0pt]
        \setcounter{enumii}{3}
      \item \label{if-kappa-phantom1}
        if $\bEv\in \phEvs_1$ then $\labelingForm(\bEv) \riff \aForm\land\labelingForm_1(\aEv)$,
      \item \label{if-kappa-phantom2} 
        if $\bEv\in \phEvs_2$ then $\labelingForm(\bEv) \riff \lnot\aForm\land\labelingForm_2(\aEv)$.
      \end{enumerate}      
    \end{enumerate}
  \end{multicols}
  \medskip

  \caption{\PwTcTITLE{} Semantics}
  \label{fig:c11}
\end{figure}
